Translation for polymorphic terms. Interpreter WIP

Ast.v
@@ -2,7 +2,7 @@ Require Template.All.
 
 Require Import Bool.
 Require Import Template.Ast Template.AstUtils.
-Require Import Template.Typing.
+Require Import Template.Typing Template.LiftSubst.
 Require Import String List.
 
 Require Import MyEnv.
@@ -24,12 +24,17 @@ Definition inductive := string.
 
 Inductive type : Set :=
 | tyInd : inductive -> type
+| tyForall : name -> type -> type
+| tyApp : type -> type -> type
+| tyVar : name -> type
+| tyRel : nat -> type
 | tyArr : type -> type -> type.
 
 Fixpoint ctor_type_to_list_anon (ty : type) : list (TC.name * type) :=
   match ty with
   | tyInd i => [(nAnon,tyInd i)]
   | tyArr ty1 ty2 => ctor_type_to_list_anon ty1 ++ ctor_type_to_list_anon ty2
+  | _ => [(nAnon,ty)] (* TODO : figure out what to do here *)
   end.
 
 Record pat := pConstr {pName : name; pVars : list name}.
@@ -48,17 +53,19 @@ Inductive expr : Set :=
 | eRel       : nat -> expr (*de Bruijn index *)
 | eVar       : name -> expr (* named variables *)
 | eLambda    : name -> type -> expr -> expr
+| eTyLam     : name -> expr -> expr (* abstraction for types *)
 | eLetIn     : name -> expr -> type -> expr -> expr
 | eApp       : expr -> expr -> expr
 | eConstr    : inductive -> name -> expr
 | eConst     : name -> expr
-| eCase      : (inductive * nat) (* # of parameters *) ->
+| eCase      : (type * nat) (* # of parameters *) ->
                type ->
                expr (* discriminee *) ->
                list (pat * expr) (* branches *) ->
                expr
 | eFix       : name (* of the fix *) -> name (* of the arg *) ->
-               type (* of the arg *) -> type (* return type *) -> expr (* body *) -> expr.
+               type (* of the arg *) -> type (* return type *) -> expr (* body *) -> expr
+| eTy        : type -> expr.
 
 (* An induction principle that takes into account nested occurrences of expressions
    in the list of branches for [eCase] *)
@@ -66,14 +73,16 @@ Definition expr_ind_case (P : expr -> Prop)
            (Hrel    : forall n : nat, P (eRel n))
            (Hvar    : forall n : name, P (eVar n))
            (Hlam    :forall (n : name) (t : type) (e : expr), P e -> P (eLambda n t e))
+           (HtyLam : forall (n : name) (e : expr), P e -> P (eTyLam n e))
            (Hletin  : forall (n : name) (e : expr),
                P e -> forall (t : type) (e0 : expr), P e0 -> P (eLetIn n e t e0))
            (Happ    :forall e : expr, P e -> forall e0 : expr, P e0 -> P (eApp e e0))
            (Hconstr :forall (i : inductive) (n : name), P (eConstr i n))
            (Hconst  :forall n : name, P (eConst n))
-           (Hcase   : forall (p : inductive * nat) (t : type) (e : expr),
+           (Hcase   : forall (p : type * nat) (t : type) (e : expr),
                P e -> forall l : list (pat * expr), Forall (fun x => P (snd x)) l ->P (eCase p t e l))
-           (Hfix    :forall (n n0 : name) (t t0 : type) (e : expr), P e -> P (eFix n n0 t t0 e)) :
+           (Hfix    :forall (n n0 : name) (t t0 : type) (e : expr), P e -> P (eFix n n0 t t0 e))
+           (Hty : forall t : type, P (eTy t)) :
   forall e : expr, P e.
 Proof.
   refine (fix ind (e : expr) := _ ).
@@ -81,6 +90,7 @@ Proof.
   + apply Hrel.
   + apply Hvar.
   + apply Hlam. apply ind.
+  + apply HtyLam. apply ind.
   + apply Hletin; apply ind.
   + apply Happ;apply ind.
   + apply Hconstr.
@@ -90,6 +100,7 @@ Proof.
     * constructor.
     * constructor. apply ind. apply IHl.
   + apply Hfix. apply ind.
+  + apply Hty.
 Defined.
 
 Fixpoint iclosed_n (n : nat) (e : expr) : bool :=
@@ -97,6 +108,7 @@ Fixpoint iclosed_n (n : nat) (e : expr) : bool :=
   | eRel i => Nat.ltb i n
   | eVar x => false
   | eLambda nm ty b => iclosed_n (1+n) b
+  | eTyLam _ b => iclosed_n (1+n) b
   | eLetIn nm e1 ty e2 => iclosed_n n e1 && iclosed_n (1+n) e2
   | eApp e1 e2 => iclosed_n n e1 && iclosed_n n e2
   | eConstr x x0 => true
@@ -106,6 +118,7 @@ Fixpoint iclosed_n (n : nat) (e : expr) : bool :=
                   (fun x => iclosed_n (length ((fst x).(pVars)) + n) (snd x)) bs in
     iclosed_n n e && bs''
   | eFix fixname nm ty1 ty2 e => iclosed_n (2+n) e
+  | eTy _ => true (* TODO : think about closed types *)
   end.
 
 Definition vars_to_apps acc vs :=
@@ -141,9 +154,9 @@ Fixpoint lookup_global ( Σ : global_env) key : option global_dec :=
   end.
 
 Definition resolve_inductive (Σ : global_env) (ind_name : ident)
-  : option (list constr) :=
+  : option (nat * list constr) :=
   match (lookup_global Σ ind_name) with
-  | Some (gdInd n _ cs _) => Some cs
+  | Some (gdInd n nparam cs _) => Some (nparam, cs)
   | None => None
   end.
 
@@ -154,7 +167,7 @@ Definition remove_proj (c : constr) := map snd (snd c).
 Definition resolve_constr (Σ : global_env) (ind_name constr_name : ident)
   : option (nat * list type)  :=
   match (resolve_inductive Σ ind_name) with
-  | Some cs => lookup_with_ind (map (fun c => (fst c, remove_proj c)) cs) constr_name
+  | Some n_cs => lookup_with_ind (map (fun c => (fst c, remove_proj c)) (snd n_cs)) constr_name
   | None => None
   end.
 
@@ -170,11 +183,30 @@ Definition bump_indices (l : list (name * nat)) (n : nat) :=
 (* For a list of vars returns a list of pairs (var,number)
 where the number is a position of the var counted from the end of the list.
  E.g. number_vars ["x"; "y"; "z"] = [("x", 2); ("y", 1); ("z", 0)] *)
-Definition number_vars (ns : list name) : list (name * nat) :=
-  combine ns (rev (seq 0 (length ns))).
+Definition number_vars (i : nat) (ns : list name) : list (name * nat) :=
+  combine ns (rev (seq i (length ns + i))).
 
-Example number_vars_xyz : number_vars ["x"; "y"; "z"] = [("x", 2); ("y", 1); ("z", 0)].
+Example number_vars_xyz : number_vars 0 ["x"; "y"; "z"] = [("x", 2); ("y", 1); ("z", 0)].
 Proof. reflexivity. Qed.
+
+Fixpoint indexify_type (l : list (name * nat)) (ty : type) : type :=
+  match ty with
+  | tyInd i => tyInd i
+  | tyForall nm ty => tyForall nm (indexify_type ((nm,0) :: bump_indices l 1) ty)
+  | tyVar nm => match (lookup l nm) with
+               | None => (* NOTE: a workaround to make the function total *)
+                 tyVar ("not a closed type")
+               | Some v => tyRel v
+               end
+  | tyRel i => tyRel i
+  | tyApp ty1 ty2 =>
+    tyApp (indexify_type l ty1) (indexify_type l ty2)
+  | tyArr ty1 ty2 =>
+    (* NOTE: we have to bump indices for the codomain,
+       since in Coq arrow also introduces a binder in a MetaCoq term.
+       So, this is purely an artifact of the translation to MetaCoq *)
+    tyArr (indexify_type l ty1) (indexify_type (bump_indices l 1) ty2)
+  end.
 
 Fixpoint indexify (l : list (name * nat)) (e : expr) : expr :=
   match e with
@@ -186,32 +218,56 @@ Fixpoint indexify (l : list (name * nat)) (e : expr) : expr :=
     | Some v => eRel v
     end
   | eLambda nm ty b =>
-    eLambda nm ty (indexify ((nm,0 ):: bump_indices l 1) b)
+    eLambda nm (indexify_type l ty) (indexify ((nm,0 ):: bump_indices l 1) b)
+  | eTyLam nm b => eTyLam nm (indexify ((nm,0 ):: bump_indices l 1) b)
   | eLetIn nm e1 ty e2 =>
-    eLetIn nm (indexify l e1) ty (indexify ((nm, 0) :: bump_indices l 1) e2)
+    eLetIn nm (indexify l e1) (indexify_type l ty) (indexify ((nm, 0) :: bump_indices l 1) e2)
   | eApp e1 e2 => eApp (indexify l e1) (indexify l e2)
   | eConstr t i as e => e
   | eConst nm as e => e
-  | eCase nm_i ty e bs =>
-    eCase nm_i ty (indexify l e)
-          (map (fun p => (fst p, indexify (number_vars (fst p).(pVars) ++
+  | eCase nm_i ty2 e bs =>
+    let (ty1,i) := nm_i in
+    eCase (indexify_type l ty1,i)
+          (indexify_type (bump_indices l 1) ty2) (indexify l e)
+          (map (fun p => (fst p, indexify (number_vars 0 (fst p).(pVars) ++
                                bump_indices l (length (fst p).(pVars))) (snd p))) bs)
   | eFix nm vn ty1 ty2 b =>
-    (* name of the fixpoint becomes an index as well *)
-    eFix nm vn ty1 ty2 (indexify ((nm,1) :: (vn,0) :: bump_indices l 2) b)
+    (* NOTE: name of the fixpoint becomes an index as well *)
+    let l' := ((nm,1) :: (vn,0) :: bump_indices l 2) in
+    (* NOTE: indexifying types is not a very good abstraction anymore.
+       [ty2] is needed in the translation in 2 places with different indices,
+       so we have to lift the indices in the translation again*)
+    let l'' := bump_indices l 1 in
+    eFix nm vn (indexify_type l ty1) (indexify_type l'' ty2) (indexify l' b)
+  | eTy ty => eTy (indexify_type l ty) (* TODO : do we want to convert to the nameless repr here? *)
   end.
 
 Fixpoint type_to_term (ty : type) : term :=
   match ty with
   | tyInd i => tInd (mkInd i 0) []
-  | tyArr t1 t2 => tProd nAnon (type_to_term t1) (type_to_term t2)
+  | tyForall nm ty => tProd (nNamed nm) (tSort Universe.type0) (type_to_term ty)
+  | tyVar nm => tVar nm
+  | tyApp ty1 ty2 => mkApps (type_to_term ty1) [type_to_term  ty2]
+  | tyArr ty1 ty2 => tProd nAnon (type_to_term ty1) (type_to_term ty2)
+  | tyRel i => tRel i
   end.
 
+Fixpoint iter_lam_type (n : nat) (t : term) :=
+  match n with
+  | O => t
+  | S n' => tLambda nAnon (tSort Universe.type0) (iter_lam_type n' t)
+  end.
 
-Fixpoint pat_to_lam (tys : list (name * type)) (body : term) : term :=
+Definition build_pat_type (tys : list term) t :=
+  tApp (iter_lam_type (length tys) t) tys.
+
+Fixpoint pat_to_lam (i : nat)(params : list term) (tys : list (name * type))
+         (body : term) : term :=
   match tys with
     [] => body
-  | (n,ty) :: tys' => tLambda (nNamed n) (type_to_term ty) (pat_to_lam tys' body)
+  | (n,ty) :: tys' =>
+    let lam_type := build_pat_type (map (lift0 i) params) (type_to_term ty) in
+    tLambda (nNamed n) lam_type (pat_to_lam (i+1) params tys' body)
   end.
 
 Fixpoint pat_to_elam (tys : list (name * type)) (body : expr) : expr :=
@@ -219,7 +275,6 @@ Fixpoint pat_to_elam (tys : list (name * type)) (body : expr) : expr :=
     [] => body
   | (n,ty) :: tys' => eLambda n ty (pat_to_elam tys' body)
   end.
-
 
 (* Resolves a pattern by looking up in the global environment
    and returns an index of the consrutor in the list of contrutors for the given iductive and
@@ -231,16 +286,17 @@ Definition resolve_pat_arity (Σ : global_env) (ind_name : name) (p : pat) : nat
   let (i, nm_tys) := from_option o_ci (0,[]) in
   (i, combine p.(pVars) nm_tys).
 
-Definition trans_branch (bs : list (pat * term))
+Definition trans_branch (params : list type)(bs : list (pat * term))
            (c : constr) :=
   let nm  := fst c in
   let tys := remove_proj c in
+  let tparams := map type_to_term params in
   let o_pt_e := find (fun x =>(fst x).(pName) =? nm) bs in
     let dummy := (0, tVar (nm ++ ": not found")%string) in
   match o_pt_e with
     | Some pt_e => if (Nat.eqb #|(fst pt_e).(pVars)| #|tys|) then
                     let vars_tys := combine (fst pt_e).(pVars) tys in
-                    (length (fst pt_e).(pVars), pat_to_lam vars_tys (snd pt_e))
+                    (length (fst pt_e).(pVars), pat_to_lam 0 tparams vars_tys (snd pt_e))
                   else (0, tVar (nm ++ ": arity does not match")%string)
     | None => dummy
   end.
@@ -248,34 +304,52 @@ Definition trans_branch (bs : list (pat * term))
 Definition fun_prod {A B C D} (f : A -> C) (g : B -> D) : A * B -> C * D :=
   fun x => (f (fst x), g (snd x)).
 
+Fixpoint decompose_inductive (ty : type) : option (name * list type) :=
+  match ty with
+  | tyInd x => Some (x,[])
+  | tyForall nm ty => None
+  | tyApp ty1 ty2 => res <- decompose_inductive ty1;;
+                     let '(ind, tys) := res in
+                     Some (ind, tys++[ty2])
+  | tyVar x => None
+  | tyRel x => None
+  | tyArr x x0 => None
+  end.
+
+
+
 Definition expr_to_term (Σ : global_env) : expr -> Ast.term :=
   fix expr_to_term e :=
   match e with
   | eRel i => tRel i
   | eVar nm => tVar nm
   | eLambda nm ty b => tLambda (nNamed nm) (type_to_term ty) (expr_to_term b)
+  | eTyLam nm b => tLambda (nNamed nm) (tSort Universe.type0) (expr_to_term b)
   | eLetIn nm e1 ty e2 => tLetIn (nNamed nm) (expr_to_term e1) (type_to_term ty) (expr_to_term e2)
   | eApp e1 e2 => mkApps (expr_to_term e1) [expr_to_term e2]
   | eConstr i t => match (resolve_constr Σ i t) with
                   | Some c => tConstruct (mkInd i 0) (fst c) []
-                  (* FIXME: a hack to make the function total *)
+                  (* NOTE: a workaround to make the function total *)
                   | None => tConstruct (mkInd (i ++ ": no declaration found.") 0) 0 []
                      end
   | eConst nm => tConst nm []
-  | eCase nm_i ty e bs =>
-    let (nm,i) := nm_i in
-    let typeInfo := tLambda nAnon (tInd (mkInd nm 0) []) (type_to_term ty) in
-    let cs := from_option (resolve_inductive Σ nm) [(nm ++ "not found",[])%string] in
+  | eCase nm_i ty2 e bs =>
+    let (ty1,i) := nm_i in
+    let (nm, tys) := from_option (decompose_inductive ty1) ("Case : not inductive", [tyVar ""]) in
+    let typeInfo := tLambda nAnon (type_to_term ty1)
+                            (type_to_term ty2) in
+    let (_,cs) := from_option (resolve_inductive Σ nm) (0,[(nm ++ "not found",[])%string]) in
     let tbs := map (fun_prod id expr_to_term) bs in
-    let branches := map (trans_branch tbs) cs in
-    (* TODO: no translation for polymorphic types, the number of parameters is zero *)
-    tCase (mkInd nm 0, 0) typeInfo (expr_to_term e) branches
+    let branches := map (trans_branch tys tbs) cs in
+    tCase (mkInd nm 0, i) typeInfo (expr_to_term e) branches
   | eFix nm nv ty1 ty2 b =>
     let tty1 := type_to_term ty1 in
     let tty2 := type_to_term ty2 in
     let ty := tProd nAnon tty1 tty2 in
-    let body := tLambda (nNamed nv) tty1 (expr_to_term b) in
+    (* NOTE: we have to lift the indices in [tty2] again, see comments in [indexify]  *)
+    let body := tLambda (nNamed nv) (lift0 1 tty1) (expr_to_term b) in
     tFix [(mkdef _ (nNamed nm) ty body 0)] 0
+  | eTy ty => type_to_term ty
   end.
 
 Definition mkArrows_rec (ind_name : name)  :=
@@ -302,41 +376,6 @@ Inductive blahh (A B : Set) :=
 Quote Recursively Definition nat_syn := nat.
 Quote Recursively Definition list_syn := list.
 Quote Recursively Definition b_syn := blahh.
-
-Compute mind_body_to_entry (
-    {|
-    TC.ind_npars := 2;
-    TC.ind_params := [{|
-                      TC.decl_name := nNamed "B";
-                      TC.decl_body := None;
-                      TC.decl_type := tSort ([] # [Level.lSet ~> false]) |};
-                     {|
-                     TC.decl_name := nNamed "A";
-                     TC.decl_body := None;
-                     TC.decl_type := tSort ([] # [Level.lSet ~> false]) |}];
-    TC.ind_bodies := [{|
-                      TC.ind_name := "blahh";
-                      TC.ind_type := tProd (nNamed "A")
-                                       (tSort ([] # [Level.lSet ~> false]))
-                                       (tProd (nNamed "B")
-                                          (tSort ([] # [Level.lSet ~> false]))
-                                          (tSort ([] # [Level.lSet ~> false])));
-                      TC.ind_kelim := [InProp; InSet; InType];
-                      TC.ind_ctors := [("bctor",
-                                       tProd (nNamed "A")
-                                         (tSort ([] # [Level.lSet ~> false]))
-                                         (tProd (nNamed "B")
-                                            (tSort ([] # [Level.lSet ~> false]))
-                                            (tProd nAnon
-                                               (tRel 1)
-                                               (tProd nAnon
-                                                  (tRel 2)
-                                                  (tApp (tRel 4) [tRel 3; tRel 2])))),
-                                       2)];
-                      TC.ind_projs := [] |}];
-    TC.ind_universes := Monomorphic_ctx (UContext.make [] ConstraintSet.empty) |}).
-
-SearchPattern (nat -> string).
 
 Definition trans_one_constr (ind_name : name) (c : constr) : term :=
   let (ctor_name, tys) := c in mkArrows ind_name tys.
@@ -392,15 +431,45 @@ Declare Custom Entry type.
 Declare Custom Entry name_type.
 
 
+Notation "[! ty !]" := ty (ty custom type at level 2).
 Notation "ty" := (tyInd ty) (in custom type at level 2, ty constr at level 3).
+
+Notation "ty1 ty2" := (tyApp ty1 ty2)
+                        (in custom type at level 4, left associativity).
+
+
 Notation "ty1 -> ty2" := (tyArr ty1 ty2)
-                           (in custom type at level 4, right associativity).
+                          (in custom type at level 4, right associativity,
+                              ty1 custom type,
+                              ty2 custom type at level 4).
+
+Notation "'∀' x , ty" := (tyForall x ty)
+                         (in custom type at level 4, right associativity,
+                             x constr at level 2,
+                             ty custom type at level 4).
+
+
+Notation " ' x " := (tyVar x)
+                    (in custom type at level 1,
+                        x constr at level 2).
+
+Notation "( x )" := x (in custom type, x custom type at level 2).
+Notation "{ x }" := x (in custom type, x constr).
+
+
+Definition ex_type := [! ∀ "A", ∀ "B", "prod" '"A" '"B" !].
+
+Compute ((type_to_term (indexify_type [] ex_type))).
+
+Make Definition ex_type_def := Eval compute in (type_to_term (indexify_type [] ex_type)).
 
 
 Notation " ctor : ty " := (ctor, removelast (ctor_type_to_list_anon ty))
                           (in custom ctor at level 2,
                               ctor constr at level 4,
                               ty custom type at level 4).
+
+
 
 (* NOTE: couldn't make this work with the recursive notation *)
 (* Notation "'data' ty_nm ':=' c1 | .. | cn ;;" := *)
@@ -533,11 +602,17 @@ Notation "'record' rec_nm := { pr1 : ty1 ; pr2 : ty2 ; pr3 : ty3 ; pr4 : ty4 ; p
 Notation "[| e |]" := e (e custom expr at level 2).
 Notation "^ i " := (eRel i) (in custom expr at level 3, i constr at level 4).
 
-Notation "\ x : ty -> b" := (eLambda x ty b)
+Notation "\ x : ty => b" := (eLambda x ty b)
                               (in custom expr at level 1,
                                   ty custom type at level 2,
                                   b custom expr at level 4,
                                   x constr at level 4).
+
+Notation "\\ A => b" := (eTyLam A b)
+                         (in custom expr at level 1,
+                             b custom expr at level 4,
+                             A constr at level 4).
+
 Notation "'let' x : ty := e1 'in' e2" := (eLetIn x e1 ty e2)
                                            (in custom expr at level 1,
                                                ty custom type at level 2,
@@ -565,19 +640,19 @@ Notation "'case' x : ty1 'return' ty2 'of' p1 -> b1 " :=
     (in custom expr at level 1,
         p1 custom pat at level 4,
         b1 custom expr at level 4,
-        ty1 constr at level 4,
+        ty1 custom type at level 4,
         ty2 custom type at level 4).
 
-Notation "'case' x : ty1 'return' ty2 'of' | p1 -> b1 | pn -> bn" :=
-  (eCase (ty1,0) ty2 x [(p1,b1);(pn,bn)])
+Notation "'case' x : ty1 # n 'return' ty2 'of' | p1 -> b1 | pn -> bn" :=
+  (eCase (ty1,n) ty2 x [(p1,b1);(pn,bn)])
     (in custom expr at level 1,
         p1 custom pat at level 4,
         pn custom pat at level 4,
         b1 custom expr at level 4,
         bn custom expr at level 4,
-        ty1 constr at level 4,
+        n constr at level 4,
+        ty1 custom type at level 4,
         ty2 custom type at level 4).
-
 
 Notation "'case' x : ty1 'return' ty2 'of' | p1 -> b1 | p2 -> b2 | p3 -> b3"  :=
   (eCase (ty1,0) ty2 x [(p1,b1);(p2,b2);(p3,b3)])
@@ -588,7 +663,17 @@ Notation "'case' x : ty1 'return' ty2 'of' | p1 -> b1 | p2 -> b2 | p3 -> b3"  :=
         b1 custom expr at level 4,
         b2 custom expr at level 4,
         b3 custom expr at level 4,
-        ty1 constr at level 4,
+        ty1 custom type at level 4,
+        ty2 custom type at level 4).
+
+Notation "'case' x : ty1 'return' ty2 'of' | p1 -> b1 | pn -> bn" :=
+  (eCase (ty1,0) ty2 x [(p1,b1);(pn,bn)])
+    (in custom expr at level 1,
+        p1 custom pat at level 4,
+        pn custom pat at level 4,
+        b1 custom expr at level 4,
+        bn custom expr at level 4,
+        ty1 custom type at level 4,
         ty2 custom type at level 4).
 
 
@@ -607,11 +692,15 @@ Notation "'fix' fixname ( v : ty1 ) : ty2 := b" := (eFix fixname v ty1 ty2 b)
 Notation "( x )" := x (in custom expr, x at level 2).
 Notation "{ x }" := x (in custom expr, x constr).
 
+
 Module StdLib.
     Definition Σ : global_env :=
     [gdInd Unit 0 [("Coq.Init.Datatypes.tt", [])] false;
       gdInd Bool 0 [("true", []); ("false", [])] false;
-     gdInd Nat 0 [("Z", []); ("Suc", [(nAnon,tyInd Nat)])] false].
+      gdInd Nat 0 [("Z", []); ("Suc", [(nAnon,tyInd Nat)])] false;
+      gdInd "list" 1 [("Nil", []); ("Cons", [(nAnon,tyRel 0);
+                                               (nAnon,tyApp (tyInd "list") (tyRel 0))])] false;
+      gdInd "prod" 2 [("Pair", [(nAnon,tyRel 1);(nAnon,tyRel 0)])] false].
 
   Notation "a + b" := [| {eConst "Coq.Init.Nat.add"} {a} {b} |]
                         (in custom expr at level 0).
@@ -645,13 +734,19 @@ Module StdLib.
   Notation "'True'" := (pConstr true_name []) (in custom pat at level 0).
   Notation "'False'" := (pConstr false_name []) ( in custom pat at level 0).
 
+  Notation "'Nil'" := (pConstr "Nil" []) (in custom pat at level 0).
+  Notation "'Cons' y z" := (pConstr "Cons" [y;z])
+                             (in custom pat at level 0,
+                                 y constr at level 4,
+                                 z constr at level 4).
+
+
   Notation "'True'" := (eConstr Bool true_name) (in custom expr at level 0).
   Notation "'False'" := (eConstr Bool false_name) ( in custom expr at level 0).
 
   Notation "'star'" :=
     (eConstr Unit "Coq.Init.Datatypes.tt")
       (in custom expr at level 0).
-
 
 End StdLib.
 
@@ -666,22 +761,22 @@ Section Examples.
 
   Check [| ^0 |].
 
-  Check [| \x : Nat -> y |].
+  Check [| \x : Nat => y |].
 
-  Definition id_f_syn :=  [| (\x : Nat -> ^0) 1 |].
+  Definition id_f_syn :=  [| (\x : Nat => ^0) 1 |].
 
   Make Definition id_f_one := Eval compute in (expr_to_term Σ id_f_syn).
   Example id_f_eq : id_f_one = 1. Proof. reflexivity. Qed.
 
   (* The same as [id_f_syn], but with named vars *)
-  Definition id_f_with_vars := [| (\x : Nat -> x) 1 |].
+  Definition id_f_with_vars := [| (\x : Nat => x) 1 |].
 
   Make Definition id_f_one' := Eval compute in (expr_to_term Σ (indexify [] id_f_with_vars)).
   Example id_f_eq' : id_f_one' = 1. Proof. reflexivity. Qed.
 
   Definition simple_let_syn :=
     [|
-     \x : Nat ->
+     \x : Nat =>
        let y : Nat := 1 in ^0
      |].
 
@@ -690,7 +785,7 @@ Section Examples.
 
   Definition simple_let_with_vars_syn :=
     [|
-     \x : Nat ->
+     \x : Nat =>
        let y : Nat := 1 in y
      |].
 
@@ -700,8 +795,8 @@ Section Examples.
 
   Definition negb_syn :=
     [|
-     \x : Bool ->
-            case x : Bool return Bool of
+     \x : Bool =>
+            case x : Bool #0 return Bool of
             | True -> False
             | False -> True
     |].
@@ -714,9 +809,41 @@ Section Examples.
   Qed.
 
   Definition myplus_syn :=
-    [| \x : Nat -> \y : Nat -> x + y |].
+    [| \x : Nat => \y : Nat => x + y |].
 
   Make Definition myplus := Eval compute in (expr_to_term Σ (indexify [] myplus_syn)).
+
+  Definition stupid_case :=
+    fun y : Set => fun x : y => fun z : list y =>
+                  match z with
+                  | [] => x
+                  | _ => x
+                  end.
+
+  Quote Definition q_stupid_case := Eval compute in stupid_case.
+  Quote Recursively Definition q_stupid_case_rec := stupid_case.
+  Quote Definition cons_syn := (fun A : Set => cons A).
+
+  Definition case_ex :=
+    [| \\y  => \x : 'y =>  \z : "list" 'y =>
+           case z : "list" 'y # 1 return 'y of
+           | Nil -> x
+           | Cons "hd" "tl" -> x |].
+
+  Compute (expr_to_term Σ (indexify [] case_ex)).
+
+  Make Definition case_ex_def := Eval compute in (expr_to_term Σ (indexify [] case_ex)).
+
+  Definition case_ex1 :=
+    [| \\y  => \"w" : 'y => \x : 'y =>  \z : "list" 'y =>
+           case z : "list" 'y # 1 return "prod" 'y 'y of
+           | Nil -> {eConstr "prod" "Pair"} {eTy (tyVar y)} {eTy (tyVar y)} x x
+           | Cons "hd" "tl" -> {eConstr "prod" "Pair"} {eTy (tyVar y)} {eTy (tyVar y)} "hd" x |].
+
+  Compute (expr_to_term Σ (indexify [] case_ex1)).
+
+  Make Definition case_ex_def1 := Eval compute in (expr_to_term Σ (indexify [] case_ex1)).
+
 
 End Examples.
 
@@ -740,6 +867,7 @@ Module Psubst.
     | eRel i => eRel (r i)
     | eVar nm  => eVar nm
     | eLambda nm ty b => eLambda nm ty (erename (↑1 ∘ r) b)
+    | eTyLam nm b => eTyLam nm (erename (↑1 ∘ r) b)
     | eLetIn nm e1 ty e2 => eLetIn nm (erename r e1) ty (erename r e2)
     | eApp e1 e2 => eApp (erename r e1) (erename r e2)
     | eConstr t i as e' => e'
@@ -750,6 +878,7 @@ Module Psubst.
                     let k := length (fst x).(pVars) in
                     (fst x, erename (↑k ∘ r) (snd x))) bs)
     | eFix nm v ty1 ty2 b => eFix nm v ty1 ty2 (erename (↑2 ∘ r) b)
+    | eTy _ => e (* should we do something here? *)
     end.
 
   Definition up (σ : psubst) := ids 0 ⋅ (erename (↑1) ∘ σ).
@@ -784,6 +913,7 @@ Module Psubst.
     | eRel i => σ i
     | eVar nm  => eVar nm
     | eLambda nm ty b => eLambda nm ty (b .[up σ])
+    | eTyLam nm b => eTyLam nm (b .[up σ])
     | eLetIn nm e1 ty e2 => eLetIn nm (e1 .[σ]) ty (e2 .[up σ])
     | eApp e1 e2 => eApp (e1 .[σ]) (e2 .[σ])
     | eConstr t i as e' => e'
@@ -792,6 +922,7 @@ Module Psubst.
       eCase nm_i ty (e .[σ])
             (map (fun x => (fst x, (snd x) .[up_k (length (fst x).(pVars)) σ])) bs)
     | eFix nm v ty1 ty2 b => eFix nm v ty1 ty2 (b .[up_k 2 σ])
+    | eTy ty => eTy ty
   end
   where "e .[ σ ]" := (apply_subst σ e).
 
