AcornMap.v
@@ -1,0 +1,218 @@
+(* Implementing a simple finite map using our embedding *)
+Require Import FMaps FMapWeakList.
+Require Import String.
+Require Import List.
+Require Import PeanoNat.
+Import ListNotations.
+From Template Require Import All.
+
+Require Import Ast CustomTactics.
+Require Import EvalE.
+
+Import MonadNotation.
+Import BaseTypes.
+Import StdLib.
+Open Scope list.
+
+
+Open Scope nat.
+
+Fixpoint mkNames (ns : list string) (postfix : string) :=
+  match ns with
+  | [] => tmPrint "Done."
+  | n :: ns' => n' <- tmEval all (n ++ postfix)%string ;;
+                  str <- tmQuote n';;
+                  tmMkDefinition n str;;
+                  mkNames ns' postfix
+  end.
+
+
+Inductive AMaybe (A : Set) :=
+| ANothing | AJust : A -> AMaybe A.
+
+Inductive AMap (A B : Set) :=
+| ANil : AMap A B | ACons : A -> B -> AMap A B -> AMap A B.
+
+Definition Σ' :=
+  Σ ++
+    [gdInd "AMaybe" 2 [("ANothing", []);  ("AJust", [(nAnon,tyRel 0)])] false;
+       gdInd "AMap" 2 [("ANil", []);  ("ACons", [(nAnon,tyRel 1);(nAnon,tyRel 0);
+                                                   (nAnon,(tyApp (tyApp (tyInd "AMap") (tyRel 1)) (tyRel 0)))])] false ].
+
+
+Definition Maybe := "AMaybe".
+Definition Map := "AMap".
+Definition MNil := "ANil".
+Definition MCons := "ACons".
+
+Run TemplateProgram
+      (mkNames ["A"; "B"; "C"; "f"; "a"; "b"; "c"; "m"; "n"; "k" ; "v"; "lookup"; "add" ] "_coq").
+
+Notation "'Nothing'" := (pConstr "ANothing" [])
+                      (in custom pat at level 0).
+
+Notation "'Nothing'" := (eConstr "AMaybe" "ANothing")
+                      (in custom expr at level 0).
+
+Notation "'Just'" := (eConstr "AMaybe" "AJust")
+                      (in custom expr at level 0).
+
+
+Notation "'MNil'" := (pConstr MNil [])
+                      (in custom pat at level 0).
+
+Notation "'MCons' x y z" := (pConstr MCons [x;y;z])
+                    (in custom pat at level 0,
+                        x constr at level 4,
+                        y constr at level 4,
+                        z constr at level 4).
+
+Notation "'MNil'" := (eConstr "AMap" "ANil")
+                      (in custom expr at level 0).
+
+Notation "'MCons'" := (eConstr "AMap" "ACons")
+                        (in custom expr at level 0).
+
+Notation " ' x " := (eTy (tyVar x))
+                    (in custom expr at level 1,
+                        x constr at level 2).
+
+Notation "'if' cond 'then' b1 'else' b2 : ty" :=
+    (eCase (tyInd Bool,0) ty cond
+           [(pConstr true_name [],b1);(pConstr false_name [],b2)])
+      (in custom expr at level 2,
+          cond custom expr at level 4,
+          ty custom type at level 4,
+          b1 custom expr at level 4,
+          b2 custom expr at level 4).
+
+
+Definition lookup_syn :=
+  [| \\A => \\B =>
+     \f : 'A -> 'A -> Bool =>
+     \k : 'A =>
+     fix lookup (m : Map 'A 'B) : Maybe 'B :=
+     case m : Map 'A 'B # 2 return Maybe 'B of
+     | MNil -> Nothing 'B
+     | MCons x y z -> if (f k x) then
+                       Just 'B y
+                       else lookup z : Maybe 'B |].
+
+Definition lookup_syn' :=
+  [| \\A => \\B =>
+     \f : 'A -> 'A -> Bool =>
+     \k : 'A =>
+     \v : 'B =>
+     fix lookup (m : Map 'A 'B) : Maybe 'B :=
+     case (MNil 'A 'B) : Map 'A 'B # 2 return Maybe 'B of
+     | MNil -> Nothing 'B
+     | MCons x y z -> if (f k x) then
+                       Just 'B y
+                       else lookup z : Maybe 'B |].
+
+
+Make Definition lookup_map := Eval compute in (expr_to_term Σ' (indexify [] lookup_syn)).
+
+
+Definition add_map_syn :=
+    [| \\A => \\B =>
+     \f : 'A -> 'A -> Bool =>
+     \k : 'A =>
+     \v : 'B =>
+     fix add (m : Map 'A 'B) : Map 'A 'B :=
+     case m : Map 'A 'B # 2 return Map 'A 'B of
+     | MNil -> MCons 'A 'B k v (MNil 'A 'B)
+     | MCons x y z -> if (f k x) then
+                       MCons 'A 'B k v z
+                     else MCons 'A 'B x y (add z) : Map 'A 'B |].
+
+Make Definition add_map := Eval compute in (expr_to_term Σ' (indexify [] add_map_syn)).
+
+Module NatMap := FMapWeakList.Make Nat_as_OT.
+
+Fixpoint from_amap {A} (m : AMap nat A) : NatMap.Raw.t A :=
+  match m with
+  | ANil _ _ => []
+  | ACons _ _ k v m' => (k,v) :: from_amap m'
+  end.
+
+Import PeanoNat.Nat.
+
+(* Showing that Acorn maps are the same as one of the Stdlib implementations
+   (we fix keys to be natural numbers) *)
+Lemma add_map_eq_stdlib {A : Set} k v m :
+  NatMap.Raw.add k v (from_amap m) = from_amap (add_map _ A PeanoNat.Nat.eqb k v m).
+Proof.
+  induction m.
+  + reflexivity.
+  + simpl in *.
+    destruct (Nat_as_OT.eq_dec k a0). subst. rewrite eqb_refl.
+    reflexivity. rewrite <- eqb_neq in n0. rewrite n0.
+    simpl. now f_equal.
+Qed.
+
+
+Module MapEval.
+
+  (* Computing with the interpreter *)
+
+  Import InterpreterEnvList.
+
+  Definition tyNat := eTy (tyInd Nat).
+
+  (* A simple example first *)
+
+  Definition case_ex1 :=
+    [| \\y  => \"w" : 'y => \x : 'y =>  \z : "list" 'y =>
+           case z : "list" 'y # 1 return "prod" 'y 'y of
+           | Nil -> {eConstr "prod" "Pair"} {eTy (tyVar y)} {eTy (tyVar y)} x "w"
+           | Cons "hd" "tl" -> {eConstr "prod" "Pair"} {eTy (tyVar y)} {eTy (tyVar y)} "hd" x |].
+
+  Make Definition case_ex_def1 := Eval compute in (expr_to_term Σ' (indexify [] case_ex1)).
+
+  Compute (expr_eval_n 20 Σ' [] ([| {case_ex1} {tyNat} 0 1 ({eConstr "list" "Nil"} {tyNat}) |])).
+
+  Definition eqb_syn :=
+    [| (fix "eqb" (n : Nat) : Nat ->  Bool :=
+           case n : Nat return Nat -> Bool of
+           | Z -> \m : Nat => (case m : Nat return Bool of
+                   | Z -> True
+                   | Suc z -> False)
+           | Suc a ->
+             \m : Nat =>
+             (case m : Nat return Bool of
+                   | Z -> False
+                   | Suc b -> "eqb" a b))
+     |].
+
+  Make Definition nat_eqb := Eval compute in (expr_to_term Σ' (indexify [] eqb_syn)).
+
+  Lemma nat_eqb_correct n m : nat_eqb n m = Nat.eqb n m.
+  Proof.
+    revert m.
+    induction n;intros m; now destruct m.
+  Qed.
+
+  Definition aMap := [| MCons {tyNat} {tyNat} 1 1 (MCons {tyNat} {tyNat} 0 0 (MNil {tyNat} {tyNat})) |].
+
+  Compute resolve_constr Σ' "AMap" "ACons".
+  Compute (expr_eval_i 20 Σ' []
+                       (indexify [] [|  {eqb_syn} 1 1 |])).
+  Compute (expr_eval_i 20 Σ' []
+                       (indexify [] [|  {aMap} |])).
+
+  Compute (expr_eval_n 20 Σ' [] ([| {lookup_syn} {tyNat} {tyNat} {eqb_syn} 0 {aMap} |])).
+
+  Compute (expr_eval_i 20 Σ' [] (indexify [] [| {lookup_syn} {tyNat} {tyNat} {eqb_syn} 0 {aMap} |])).
+
+  Compute (expr_eval_i 20 Σ' []
+                       (indexify [] [| {add_map_syn} {tyNat} {tyNat} {eqb_syn} 0 1 (MNil {tyNat} {tyNat}) |])).
+
+  Definition zzz := [| \\A => \x : ∀ B, 'B -> 'A => x |].
+
+  Make Definition zzzzz := Eval compute in (expr_to_term Σ' (indexify [] zzz)).
+
+  Compute (expr_eval_i 20 Σ' []
+                       (indexify [] [| {zzz} {tyNat} (\\B => \x :'B => 0)|])).
+
+  End MapEval.
