EnvSubst.v
@@ -1,0 +1,169 @@
+(** * Convertion from values back to expressions through the environment substitution *)
+Require Import List.
+
+Require Import Ast.
+Require Import EvalE.
+Require Import MyEnv.
+
+Import InterpreterEnvList.
+
+(* TODO: add support for polymorphism *)
+
+(* Substitution for the named representation *)
+(* NOTE: assumes, that expression in [ρ] are closed! *)
+ Fixpoint subst_env (ρ : list (name * expr)) (e : expr) : expr :=
+  match e with
+  | eRel i as e' => e'
+  | eVar nm  => match lookup ρ nm with
+                    | Some v => v
+                    | None => e
+                    end
+  | eLambda nm ty b => eLambda nm ty (subst_env (remove_by_key nm ρ) b)
+  | eTyLam nm b => eTyLam nm (subst_env (remove_by_key nm ρ) b)
+  | eLetIn nm e1 ty e2 => eLetIn nm (subst_env ρ e1) ty (subst_env (remove_by_key nm ρ) e2)
+  | eApp e1 e2 => eApp (subst_env ρ e1) (subst_env ρ e2)
+  | eConstr t i as e' => e'
+  | eConst nm => eConst nm
+  | eCase nm_i ty e bs =>
+    (* TODO: this case is not complete! We ignore variables bound by patterns *)
+    eCase nm_i ty (subst_env ρ e) (map (fun x => (fst x, subst_env ρ (snd x))) bs)
+  | eFix nm v ty1 ty2 b => eFix nm v ty1 ty2 (subst_env (remove_by_key v ρ) b)
+  | eTy _ => e
+  end.
+
+
+ (* Substitution for the nameless representation *)
+
+  (* NOTE: assumes, that expression in [ρ] are closed! *)
+ Fixpoint subst_env_i_aux (k : nat) (ρ : env expr) (e : expr) : expr :=
+  match e with
+  | eRel i => if Nat.leb k i then
+               from_option (lookup_i ρ (i-k)) (eRel i) else eRel i
+  | eVar nm  => eVar nm
+  | eLambda nm ty b => eLambda nm ty (subst_env_i_aux (1+k) ρ b)
+  | eLetIn nm e1 ty e2 => eLetIn nm (subst_env_i_aux k ρ e1) ty (subst_env_i_aux (1+k) ρ e2)
+  | eApp e1 e2 => eApp (subst_env_i_aux k ρ e1) (subst_env_i_aux k ρ e2)
+  | eConstr t i as e' => e'
+  | eConst nm => eConst nm
+  | eCase nm_i ty e bs =>
+    eCase nm_i ty (subst_env_i_aux k ρ e)
+          (map (fun x => (fst x, subst_env_i_aux (length (fst x).(pVars) + k) ρ (snd x))) bs)
+  | eFix nm v ty1 ty2 b => eFix nm v ty1 ty2 (subst_env_i_aux (2+k) ρ b)
+  end.
+
+ Definition subst_env_i := subst_env_i_aux 0.
+
+  (* Converting from values back to expression.
+     This will be used to compare results of the evaluation with different semantics, or
+     for stating soundness theorem for the translation to a different language, e.g.
+     to Template Coq terms.
+
+     The most non-trivial part is to convert closures, for which we have to perform some form
+     of substitution of values from the value environment (see [subst_env])
+     Inspired by the implementation of
+     "A Certified Implementation of ML with Structural Polymorphism" by Jacques Garrigue.
+   *)
+  Fixpoint from_val (v : val) : expr :=
+    match v with
+    | vConstr x i vs => vars_to_apps (eConstr x i) (map from_val vs)
+    | vClos ρ nm cm ty1 ty2 e =>
+      let res := match cm with
+                 | cmLam => eLambda nm ty1 e
+                 | cmFix fixname => eFix fixname nm ty1 ty2 e
+                 end
+      in subst_env (map (fun x => (fst x, from_val (snd x))) ρ) res
+    end.
+
+  Definition inst_env (ρ : env val) (e : expr) : expr :=
+    subst_env (map (fun x => (fst x, from_val (snd x))) ρ) e.
+
+  Fixpoint from_val_i (v : val) : expr :=
+    match v with
+    | vConstr x i vs => vars_to_apps (eConstr x i) (map from_val_i vs)
+    | vClos ρ nm cm ty1 ty2 e =>
+      let res := match cm with
+                 | cmLam => eLambda nm ty1 e
+                 | cmFix fixname => eFix fixname nm ty1 ty2 e
+                end
+     in subst_env_i (map (fun x => (fst x, from_val_i (snd x))) ρ) res
+   end.
+
+  (* The similar notation will be used when we change to a parallel substitution *)
+  Notation "e .[ ρ ] n " := (subst_env_i_aux n ρ e) (at level 50).
+
+ Definition inst_env_i (ρ : env val) (e : expr) : expr :=
+   subst_env_i (map (fun x => (fst x, from_val_i (snd x))) ρ) e.
+ Notation "e .[ ρ ]" := (subst_env_i ρ e) (at level 50).
+
+ Module Equivalence.
+   Reserved Notation "v1 ≈ v2" (at level 50).
+
+   Inductive val_equiv : relation val :=
+   | veqConstr i n (vs1 vs2 : list val) :
+       Forall2 (fun v1 v2 => v1 ≈ v2) vs1 vs2 -> vConstr i n vs1 ≈ vConstr i n vs2
+   | veqClosLam ρ1 ρ2 nm ty1 e1 e2 :
+       inst_env_i ρ1 (eLambda nm ty1 e1) = inst_env_i ρ2 (eLambda nm ty1 e2) ->
+       (* ty2 used only by a fixpoint, so it doesn't matter here *)
+       forall ty2 ty2', vClos ρ1 nm cmLam ty1 ty2 e1 ≈ vClos ρ2 nm cmLam ty1 ty2' e2
+   | veqClosFix ρ1 ρ2 n ty1 ty2 e1 e2 :
+       (forall fixname ty2 , inst_env_i ρ1 (eFix fixname n ty1 ty2 e1) =
+       inst_env_i ρ2 (eFix fixname n ty1 ty2 e2)) ->
+       (forall fixname, vClos ρ1 n (cmFix fixname) ty1 ty2 e1 ≈ vClos ρ2 n (cmFix fixname) ty1 ty2 e2)
+   where
+   "v1 ≈ v2" := (val_equiv v1 v2).
+
+   Definition list_val_equiv vs1 vs2 := Forall2 (fun v1 v2 => v1 ≈ v2) vs1 vs2.
+   Notation " vs1 ≈ₗ vs2 " := (list_val_equiv vs1 vs2) (at level 50).
+
+   Instance val_equiv_reflexive : Reflexive val_equiv.
+   Proof.
+     intros v. induction v using val_ind_full.
+     + constructor.
+       induction l;constructor; inversion H; easy.
+     + destruct cm;constructor;reflexivity.
+   Defined.
+
+   (* TODO:  Add the rest to prove that [val_equiv] is indeed an equivalence *)
+   Axiom val_equiv_symmetric : Symmetric val_equiv.
+   Axiom val_equiv_transitive : Transitive val_equiv.
+
+   Existing Instance val_equiv_symmetric.
+   Existing Instance val_equiv_transitive.
+
+   (* TODO:  Define these  *)
+   Axiom list_val_equiv_reflexive : Reflexive list_val_equiv.
+   Axiom list_val_equiv_symmetric : Symmetric list_val_equiv.
+   Axiom list_val_equiv_transitive : Transitive list_val_equiv.
+
+   Existing Instance list_val_equiv_reflexive.
+   Existing Instance list_val_equiv_symmetric.
+   Existing Instance list_val_equiv_transitive.
+
+   Lemma list_val_compat v1 v2 vs1 vs2 :
+     v1 ≈ v2 -> vs1 ≈ₗ vs2 -> (v1 :: vs1) ≈ₗ (v2 :: vs2).
+   Proof.
+     intros Heq Heql.
+     constructor;easy.
+   Qed.
+
+   Instance cons_compat : Proper (val_equiv ==> list_val_equiv ==> list_val_equiv) cons.
+   Proof.
+      cbv;intros;apply list_val_compat;assumption.
+    Defined.
+
+    Lemma constr_cons_compat (vs1 vs2 : list val) (i : inductive) (nm : name) :
+      vs1 ≈ₗ vs2 -> (vConstr i nm vs1) ≈ (vConstr i nm vs2).
+    Proof.
+      intros Heql.
+      constructor.
+      induction Heql.
+      + constructor.
+      + constructor; assumption.
+    Defined.
+
+    Instance constr_morph i nm : Proper (list_val_equiv ==> val_equiv) (vConstr i nm).
+    Proof.
+      cbv;intros;apply constr_cons_compat;assumption.
+    Defined.
+
+  End Equivalence.
